\documentclass[fontsize=9p]{article}

\usepackage{a4}
\usepackage{latexsym}
\usepackage{pncproofmacros}
\usepackage{color}
\usepackage{amssymb}

\setlength{\textheight}{225mm}	   
\setlength{\topmargin}{-12mm}	  


\title{Software Testing \& Verification Proof Assignment}
\author{Jarno Le Cont\'{e} \hspace{2mm} 3725154 \\ \noindent Bas Meesters \hspace{2mm} 3700569}

% Program without breaks
\begin{document}
\maketitle
\section* {Task 1}
\textbf {Simple variant:}
\vspace {2mm} \\
\{$*N \ge 0 \wedge sorted \: a \: N *$\} \\ \\
found := false; \\
 i := 0; \\
while i $<$ N do \{ found := found $\vee$ (a[i]=x) ; i:= i+1\} \\ \\
 {\color{blue} \{*return=(i=N $\wedge$ found =  ($\exists i : 0 \le i < N : a[i] = x))*$\}}

% Program with breaks
\vspace{5 mm}
\noindent \textbf {Variant with breaks:} \\
\vspace {2 mm}
\{*$N \ge 0 \wedge sorted \: a \: N $*\} \\ \\
 found := false; \\
i := 0;\\
while $i < N \wedge \neg found \wedge a[i] \le x \:do \: \{$\\
\indent found := found $\vee (a[i]=x);$\\
\indent  i := i + 1\\
 \}\\ \\
{\color{blue} \{*return=($0 \le i \le N \wedge $ found =  ($\exists i : 0 \le i < N : a[i] = x))*$\}} 
\vspace{5 mm}

\noindent \textbf {Extra note:} \\
Because no write-operations are made on the arrays, it is assumed they never change their order and therefore remain sorted
\section* {Task 2}
%Too prove: \\
%\indent INIT: \hspace{3mm} $ \models P \Rightarrow I$ \\
%\indent PIC: \hspace{3mm}  $\{* I \wedge  g *\} \: S \: \{*I*\}$ \\
%\indent PEC: \hspace{3mm} $ \models I \wedge \neg g \Rightarrow Q$ \\  

\noindent Invariant (I): \\
$\{* 0 \le i \le N \wedge (found = (\exists k : 0\le k < i : a[k] = x)) \wedge sorted \:a \:N *\}$ \\ \\

\noindent Statement S is a sequence S1;S2 \\
S1: found := found $\vee$ (a[i] = x); \\
S2: i := i + 1;  \\\\

\noindent Guard g:\\
\{ * i $<$ N * \} \\

\noindent \begin{PROOF}{ PEC} \\
 \ASSUME {A1} {found = (\exists k : 0 \le k < i : a[k]=x)} \\
\ASSUME {A2} {0 \le i \le N} \\
\ASSUME {A3} {i \ge N} \\
\GOAL {G} {(i = N) \wedge (found = (\exists k : 0 \le k < N : a[k] =x) } \\
\begin{BODY}
\item[1.] \HINT {combine A2 and A3} \\
\EXPR {i = N}
\item[2.] \HINT {from 1 replace i with N in A1} \\
\EXPR {(found = (\exists k : 0 \le k < N : a[k] =x))}
\item[3.] \HINT {combine 1 and 2} \\
\EXPR {(i = N) \wedge (found = (\exists k : 0 \le k < N : a[k] = x))}
\end{BODY}
\end{PROOF}
\vspace{5mm}

\noindent \begin{PROOF}{PIC}  \\
PIC: $\{* I \wedge  g *\} \: S \: \{*I*\}$ \\ 
\noindent\ASSUME{A1}{found = (\exists k : 0\le k < i : a[k] = x) } \\
\ASSUME{A2} {0 \le i < N } \\
\GOAL{G1}{wp \: S \: I} %// note: check if this is the weakest-precondition

\begin{BODY}

\item[1.] \HINT{see calculate wp} 
	
	\EXPR{wp \:S \: I = 0 \le i + 1 \le N \wedge ((found \vee a[i]=x) = (\exists k : 0 \le k < i + 1: a[k] =x))} \\

\begin{PROOF}{ calculate wp}\\
\begin{BODY}
\item[] \EXPR {wp (found := found \vee a[i] =x; i := i + 1) (0 \le i \le N \wedge (found = (\exists k : 0\le k < i : a[k] = x)))}
\item[1.] \HINT { wp of statements sequence} \\
	\EXPR { wp (found := found \vee a[i] =x) (wp (i := i + 1) (0 \le i \le N \wedge (found = (\exists k : 0\le k < i : a[k] = x))) }
\item[2.] \HINT {wp of assignment} \\
\EXPR{wp (found := found \vee a[i]=x) (0 \le i + 1 \le N \wedge (found = (\exists k : 0\le k < i + 1 : a[k] = x)))}
\item[3.] \HINT {wp of assignment} \\
\EXPR {0 \le i + 1 \le N \wedge ((found \vee a[i] =x) =  (\exists k : 0\le k < i + 1 : a[k] = x)) }
\end{BODY}
\end{PROOF}

\item[2] \HINT{see subproof equality} \\
	\EXPR{\exists k: 0 \le k < i : a[k] =x) \vee (a[i] =x) =  (\exists k : 0\le k < i +1: a[k] = x)} 
\vspace{4mm} \\
\begin{PROOF} {equality}
\item[] \EXPR {[some \: i]} 
\item[] \EXPR {[some \: x]} \\
\ASSUME {A1} {(\exists k : 0\le k < i: a[k] = x) \vee (a[i] = x)} \\
\GOAL {G} {(\exists k : 0\le k < i: a[k] = x) \vee (a[i] = x) = (\exists k : 0\le k < i +1: a[k] = x) } \\
\begin{BODY}
\item[] \EXPR {(\exists k : 0\le k < i: a[k] = x) \vee (a[i] = x)} 
\item [1.] \HINT {introduce  $\exists$ -quantor } \\
\EXPR {(\exists k : 0\le k < i: a[k] = x) = (\exists k : k =i : a[k] = x)}
\item[2.] \HINT {combine domains} \\
\EXPR {(\exists k : 0 \le k < i + 1: a[k] = x)}
\item[3.] \HINT {we have proven equality} \\
\EXPR  {(\exists k : 0\le k < i: a[k] = x) \vee (a[i] = x) = (\exists k : 0\le k < i +1: a[k] = x) }

\end{BODY}
\end{PROOF}

\item[3.] \HINT{ reversed substitution of A1 in 2} \\
	\EXPR{((found \vee a[i] = x) =  (\exists k : 0\le k < i +1: a[k] = x))}

\item[4.] \HINT{rewrite A2} \\
	\EXPR{ 0 \le i + 1 \le N}

\item[5.] \HINT{combine 3 and 4} \\
	\EXPR{ 0 \le i + 1 \le N \wedge ((found \vee a[i] = x) =  (\exists k : 0\le k < i +1: a[k] = x) }

\item[6.] \HINT {by equility on 1 and 5 we have proven wp} \\
\EXPR {wp \:S \:I =  0 \le i + 1 \le N \wedge(( found \vee a[i] = x) =  (\exists k : 0\le k < i +1: a[k] = x)) } \\
\end{BODY}
\end{PROOF} 
\vspace {5mm}

\noindent \begin{PROOF} {PTC1} \\
Termination metric is N - i \\
\ASSUME {A1} {i \le N} \\
\GOAL {G} { N - i \ge 0} \\
\begin{BODY}
\item \HINT {follows from A1} \\
\EXPR { N - i \ge 0}
\end{BODY}
\end{PROOF} 
\vspace{5mm}

\noindent \begin{PROOF} {PTC2} \\
\ASSUME {A1} { found = (\exists i : 0 \le i < N : a[i] = x)} \\
\ASSUME {A2} {i \le N } \\
\ASSUME {D1} {Q = wp(C:= m) \: body \:(N - i < C) \: i := 0} \\
\GOAL {G} { Q}
\begin{BODY}
\item[1.] \HINT {calculating wp} \\
\EXPR {N - i  < C}
\item[2.] \HINT {i := i + 1; C := N - i} \\
\EXPR {N - (i+ i)  <  N - i}
\item[3.] \HINT { rewrite} \\
\EXPR { N - i - 1 < N - i}
\item[4.] \HINT {follows from 1,2 and 3} \\
\EXPR {Q}
\end{BODY}
\end{PROOF}
\vspace{5mm}

\noindent \begin{PROOF} {Init} \\
\ASSUME {A1} {N \ge 0} \\
\ASSUME {A2} {sorted \:a \:N} \\
\GOAL {G} {wp = (found := false;  i := 0 ) \: I} \\
\begin{BODY}
\item \HINT {calculate wp} \\
\EXPR { found = (\exists i : 0 \le i < N : a[i] = x)}
\item \HINT {follows from intialisation} \\
\EXPR { found := false; i := 0}
\item \HINT {follows from 1 and 2} \\
\EXPR {wp}
\end{BODY}
\end{PROOF} 
\vspace{5mm}

\section*{Task 3}
\noindent Invariant (I): \\
$\{* 0 \le i \le N \wedge (found = (\exists k : 0\le k < i : a[k] = x)) \wedge sorted \:a \:N *\}$ \\ \\

\noindent Statement S is a sequence S1;S2 \\
S1: found := found $\vee$ (a[i] = x); \\
S2: i := i + 1;  \\\\

\noindent Guard g:\\
\{ * i $<$ N $\wedge \neg$ found $\wedge$ a[i] $\le$ x * \} \\

\noindent \begin{PROOF} {PEC} \\
\ASSUME {A1} {(found = ( \exists k : 0 \le k < i : a[k] = x))} \\
\ASSUME {A2} {0 \le i \le N} \\
\ASSUME{A3} {i \ge N \vee found \vee  a[i] > x} \\
\ASSUME{A4} {(\forall i : 0 \le i < N : ( \forall j : i \le j < N : a[i] \le a[j]))} \\
\GOAL {G} {0 \le i \le N \wedge (found = (\exists k : 0 \le k < N : a[k] = x))} \\
\begin{BODY}
\item[1.] \HINT {see subproof breakWithCounter} \\
\EXPR {i \ge N \Rightarrow 0 \le i \le N \wedge (found = (\exists k : 0 \le k < N : a[k] = x))} \\ \\
\begin{PROOF}{breakWithCounter} \\
\ASSUME{A1} { found = (\exists k : 0 \le k < i : a[k] = x)} \\
\ASSUME{A2} {i \ge N} \\
\ASSUME{A3} {0 \le i \le N} \\
\GOAL {G} { 0 \le i \le N \wedge (found = (\exists k : 0 \le k < N : a[k] = x))} \\
\begin{BODY}
\item[1.] \HINT {combine A2 and A3} \\
\EXPR {i = N}
\item[2.] \HINT {replace in A1 with N} \\
\EXPR {found = (\exists k : 0 \le k < N : a[k] = x)}
\item[3.] \HINT{combine A3 and 2} \\
\EXPR {0 \le i \le N \wedge (found = (\exists k : 0 \le k < N : a[k] = x))} \\
\end{BODY}
\end{PROOF} 
\vspace {3mm}

\item[2.] \HINT {see subproof breakWithFound} \\
\EXPR {found \Rightarrow 0 \le i \le N \wedge (found = (\exists k : 0 \le k < i : a[k] = x))} \
\vspace{3mm}
\begin{PROOF} {breakWithFound} \\
\ASSUME{A1} {found = (\exists k : 0 \le k < N : a[k] = x)} \\
\ASSUME{A2} {found} \\
\ASSUME{A3} {0 \le i \le N} \\
\GOAL{G} {0 \le i \le N \wedge (found = (\exists k : 0 \le k < N : a[k] = x))} \\
\begin{BODY}
\item[1.] \HINT {substitute found in A1 with A2} \\
\EXPR {(\exists k : 0 \le k < i : a[k] = x)}
\item[2.] \HINT {domain expanding} \\
\EXPR {(\exists k : 0 \le k < i \vee i \le k < N : a[k] = x)}
\item[3.] \HINT{domain combine} \\
\EXPR { (\exists k : 0 \le k < N : a[k] = x)}
\item[4.] \HINT {equality of 3 and A2} \\
\EXPR {found = (\exists k : 0 \le k < N : a[k] = x))}
\item[5.] \HINT {combine with A3} \\
\EXPR {0 \le i \le N \wedge (found = (\exists k : 0 \le k < N : a[k] = x))} \\
\end{BODY}
\item[3.] \HINT {see subproof breakWithValue} \\
\EXPR {a[i] > x \Rightarrow 0 \le i \le N \wedge (found = (\exists k : 0 \le k < N : a[k] = x))} 
\vspace{3 mm}

\begin{PROOF} {breakWithValue} \\
\ASSUME {A1} {found = (\exists k : 0 \le k < i : a[k] = x)} \\
\ASSUME{A2} {a[i] > x} \\
\ASSUME{A3} {0 \le i \le N} \\
\ASSUME{A4} {(\forall i : 0 \le i < N : (\forall j : i \le j < N : a[i] \le a[j]))} \\
\GOAL{G} {0 \le i \le N \wedge (found = (\exists k : 0 \le k < N : a[k] = x))} \\
\begin{BODY} 
\item[1.] \HINT {kwantor elimination in A4} [ANY i]\\
\EXPR {0 \le i < N \Rightarrow (\forall j : i \le j < N : a[i] \le a[j])}
\item[2.] \HINT {follows from A3 and 1} \\
\EXPR {(\forall j : i \le j < N : a[i] \le a[j])}
\item[3.] \HINT {follows from 2 and A2} \\
\EXPR{\neg (\exists j : i \le j < N : a[j] = x)}
\item[4.] \HINT {flip domain of 3} \\
\EXPR{(\exists j : j < i \vee j \ge N : a[j] = x)}
\item[5.] \HINT {split kwantor from 4} \\
\EXPR {(\exists j : j < i \vee :a[j] = x) \vee (\exists j : j \ge N : a[j] = x)}
\item[6.] \HINT {remove second part from 5} \\
\EXPR { (\exists j :j < i  : a[j] = x)}
\item[7.] \HINT {follows from equality of 6 and A1} \\
\EXPR { (found = (\exists k : 0 \le k < i : a[k] = x))}
\item[8.] \HINT {combine with 7 and A3} \\
\EXPR {0 \le i \le N \wedge (found = (\exists k : 0 \le k < N : a[k] = x))}
\end{BODY}
\end{PROOF}
\item[4.] \HINT {A3 with 1,2 and 3 will prove G} \\
\EXPR {0 \le i \le N \wedge (found = (\exists k : 0 \le k < N : a[k] = x))}
\end{PROOF}
\end{BODY}
\end{PROOF}
\vspace {5mm}
\noindent \begin{PROOF}{PIC}  \\
PIC: $\{* I \wedge  g *\} \: S \: \{*I*\}$ \\ 
\noindent\ASSUME{A1}{found = (\exists k : 0\le k < i : a[k] = x) } \\
\ASSUME{A2} {0 \le i < N } \\
\GOAL{G1}{wp \: S \: I} %// note: check if this is the weakest-precondition

\begin{BODY}

\item[1.] \HINT{see calculate wp} 
	
	\EXPR{wp \:S \: I = 0 \le i + 1 \le N \wedge ((found \vee a[i]=x) = (\exists k : 0 \le k < i + 1: a[k] =x))} \\

\begin{PROOF}{ calculate wp}\\
\begin{BODY}
\item[] \EXPR {wp (found := found \vee a[i] =x; i := i + 1) (0 \le i \le N \wedge (found = (\exists k : 0\le k < i : a[k] = x)))}
\item[1.] \HINT { wp of statements sequence} \\
	\EXPR { wp (found := found \vee a[i] =x) (wp (i := i + 1) (0 \le i \le N \wedge (found = (\exists k : 0\le k < i : a[k] = x))) }
\item[2.] \HINT {wp of assignment} \\
\EXPR{wp (found := found \vee a[i]=x) (0 \le i + 1 \le N \wedge (found = (\exists k : 0\le k < i + 1 : a[k] = x)))}
\item[3.] \HINT {wp of assignment} \\
\EXPR {0 \le i + 1 \le N \wedge ((found \vee a[i] =x) =  (\exists k : 0\le k < i + 1 : a[k] = x)) }
\end{BODY}
\end{PROOF}

\item[2] \HINT{see subproof equality} \\
	\EXPR{\exists k: 0 \le k < i : a[k] =x) \vee (a[i] =x) =  (\exists k : 0\le k \le i +1: a[k] = x)} 
\vspace{4mm} \\
\begin{PROOF} {equality}
\item[] \EXPR {[some \: i]} 
\item[] \EXPR {[some \: x]} \\
\ASSUME {A1} {(\exists k : 0\le k < i: a[k] = x) \vee (a[i] = x)} \\
\GOAL {G} {\exists k : 0\le k < i: a[k] = x) \vee (a[i] = x) = (\exists k : 0\le k < i +1: a[k] = x) } \\
\begin{BODY}
\item[] \EXPR {\exists k : 0\le k < i: a[k] = x) \vee (a[i] = x)} 
\item [1.] \HINT {introduce  $\exists$ -quantor } \\
\EXPR {(\exists k : 0\le k < i: a[k] = x) = (\exists k : k =i : a[k] = x)}
\item[2.] \HINT {combine domains} \\
\EXPR {(\exists k : 0 \le k < i + 1: a[k] = x)}
\item[3.] \HINT {we have proven equality} \\
\EXPR  {(\exists k : 0\le k < i: a[k] = x) \vee (a[i] = x) = (\exists k : 0\le k < i +1: a[k] = x) }

\end{BODY}
\end{PROOF}

\item[3.] \HINT{ reversed substitution of A1 in 2} \\
	\EXPR{((found \vee a[i] = x) =  (\exists k : 0\le k < i +1: a[k] = x))}

\item[4.] \HINT{rewrite A2} \\
	\EXPR{ 0 \le i + 1 \le N}

\item[5.] \HINT{combine 3 and 4} \\
	\EXPR{ 0 \le i + 1 \le N \wedge ((found \vee a[i] = x) =  (\exists k : 0\le k < i +1: a[k] = x) }

\item[6.] \HINT {by equility on 1 and 5 we have proven wp} \\
\EXPR {wp \:S \:I =  0 \le i + 1 \le N \wedge(( found \vee a[i] = x) =  (\exists k : 0\le k < i +1: a[k] = x)) } \\
\end{BODY}
\end{PROOF} 

\end{document}
